code/hash-new/Hacl.Hash.fst
@@ -56,18 +56,18 @@ let mk_update_multi a update s blocks n_blocks =
   assert (B.length blocks = U32.v n_blocks * size_block a);
   C.Loops.for 0ul n_blocks inv f
 
-let update_multi_sha2_224: update_multi_t SHA2_224 =
+let update_multi_sha2_224: update_multi_st SHA2_224 =
   Tactics.(synth_by_tactic
     (specialize (mk_update_multi SHA2_224 Hacl.SHA2.update_224) [`%mk_update_multi]))
 
-let update_multi_sha2_256: update_multi_t SHA2_256 =
+let update_multi_sha2_256: update_multi_st SHA2_256 =
   Tactics.(synth_by_tactic
     (specialize (mk_update_multi SHA2_256 Hacl.SHA2.update_256) [`%mk_update_multi]))
 
-let update_multi_sha2_384: update_multi_t SHA2_384 =
+let update_multi_sha2_384: update_multi_st SHA2_384 =
   Tactics.(synth_by_tactic
     (specialize (mk_update_multi SHA2_384 Hacl.SHA2.update_384) [`%mk_update_multi]))
 
-let update_multi_sha2_512: update_multi_t SHA2_512 =
+let update_multi_sha2_512: update_multi_st SHA2_512 =
   Tactics.(synth_by_tactic
     (specialize (mk_update_multi SHA2_512 Hacl.SHA2.update_512) [`%mk_update_multi]))
